demo/fib/Fib45proof.v
@@ -1,0 +1,147 @@
+Require Import CoqlibC Maps Postorder.
+Require Import AST Linking.
+Require Import ValuesC MemoryC GlobalenvsC Events Smallstep.
+Require Import Op ClightC.
+Require Import CtypesC CtypingC.
+Require Import sflib.
+Require Import IntegersC.
+
+Require Import Simulation.
+Require Import Skeleton Mod ModSem SimMod SimModSemLift SimSymb SimMemLift MatchSimModSemExcl.
+Require SoundTop.
+Require SimMemId.
+Require Import Any.
+Require Import SIR.
+Require Import SIRStack.
+Require Import Fib5.
+Require Import Fib4.
+Require Import ModSemProps.
+Require Import Program.
+Require Import SIRProps.
+
+Set Implicit Arguments.
+
+
+
+
+
+
+Ltac step := gstep; econs; et.
+Ltac step_assume := match goal with
+                    | |- context[assume ?P ;; _] =>
+                      (*** I want to unfold only the "first" assume.
+Maybe we should use notation instead, so that we can avoid this weird "unfold"? ***)
+                      first[
+                          unfold assume at 5|
+                          unfold assume at 4|
+                          unfold assume at 3|
+                          unfold assume at 2|
+                          unfold assume at 1|
+                          unfold assume at 0
+                        ];
+                      let name := fresh "T" in
+                      destruct (ClassicalDescription.excluded_middle_informative P) as [name|name]; cycle 1; [
+                        unfold triggerUB; rewrite bind_vis (*** <---------- this is counter-intuitive. Any good idea? ***);
+                        try step|]
+                    end
+.
+Ltac step_unwrapN := match goal with
+                     | |- context[unwrapN ?ox ;; _] =>
+                       (*** I want to unfold only the "first" assume.
+Maybe we should use notation instead, so that we can avoid this weird "unfold"? ***)
+                       first[
+                           unfold unwrapN at 5|
+                           unfold unwrapN at 4|
+                           unfold unwrapN at 3|
+                           unfold unwrapN at 2|
+                           unfold unwrapN at 1|
+                           unfold unwrapN at 0
+                         ];
+                       let name := fresh "T" in
+                       destruct ox eqn:name; cycle 1
+                     end
+.
+Ltac step_guaranteeK := match goal with
+                        | |- context[guaranteeK ?P ;; _] =>
+                          (*** I want to unfold only the "first" assume.
+Maybe we should use notation instead, so that we can avoid this weird "unfold"? ***)
+                          first[
+                              unfold guaranteeK at 5|
+                              unfold guaranteeK at 4|
+                              unfold guaranteeK at 3|
+                              unfold guaranteeK at 2|
+                              unfold guaranteeK at 1|
+                              unfold guaranteeK at 0
+                            ];
+                          destruct (ClassicalDescription.excluded_middle_informative P); cycle 1
+                        | |- context[guaranteeK ?P ?Q] =>
+                          (*** I want to unfold only the "first" assume.
+Maybe we should use notation instead, so that we can avoid this weird "unfold"? ***)
+                          first[
+                              unfold guaranteeK at 5|
+                              unfold guaranteeK at 4|
+                              unfold guaranteeK at 3|
+                              unfold guaranteeK at 2|
+                              unfold guaranteeK at 1|
+                              unfold guaranteeK at 0
+                            ];
+                          destruct (ClassicalDescription.excluded_middle_informative (P Q)); cycle 1
+                        end
+.
+Ltac step_guarantee := match goal with
+                    | |- context[guarantee ?P ;; _] =>
+                      (*** I want to unfold only the "first" guarantee.
+Maybe we should use notation instead, so that we can avoid this weird "unfold"? ***)
+                      first[
+                          unfold guarantee at 5|
+                          unfold guarantee at 4|
+                          unfold guarantee at 3|
+                          unfold guarantee at 2|
+                          unfold guarantee at 1|
+                          unfold guarantee at 0
+                        ];
+                      let name := fresh "T" in
+                      destruct (ClassicalDescription.excluded_middle_informative P) as [name|name]; cycle 1; [
+                        unfold triggerNB; rewrite bind_vis (*** <---------- this is counter-intuitive. Any good idea? ***);
+                        try step|]
+                    end
+.
+
+
+
+
+
+
+Definition mp: ModPair.t := SimSymbId.mk_mp (Fib5.module) (Fib4.module).
+
+Local Opaque ident_eq.
+Theorem sim_mod: ModPair.sim mp.
+Proof.
+  assert(tau: forall E R (a: itree E R), (tau;; a) = a).
+  { admit "backdoor --- relax sim_st to allow tau* before each progress". }
+  eapply SimSIRLocal.sim_mod with (SO := eq); ss.
+  ii. clarify. unfold Fib5.prog, prog. ss. des_ifs; econs; et.
+  { r. ii. clarify.
+    assert(EQ: (Fib5.f_fib_ru oh_tgt m vs) = (f_fib_ru oh_tgt m vs)).
+    { refl. }
+    admit "refl".
+  }
+  ginit.
+  { i. eapply cpn2_wcompat; eauto with paco. }
+  ii; clarify.
+  unfold Fib5.f_fib, f_fib.
+  replace Fib5.precond with precond by ss.
+  step_assume.
+  { unfold assume. des_ifs. unfold triggerUB. irw. step. }
+  unfold assume. des_ifs.
+  irw. step.
+  ii. rr in H. des_ifs. des. clarify.
+  unfold guaranteeK. des_ifs; cycle 1.
+  { step. }
+
+  rewrite <- tau. rewrite <- tau.
+  step. eexists (exist _ _ _). cbn.
+  step.
+Unshelve.
+  cbn. des_ifs.
+Qed.
