specIR/SIRProps.v
@@ -1,3 +1,4 @@
 Require Export SIRStackproof.
+Require Export SIRHoareproof.
 Require Export SimSIR.
 Require Export SimSIRLocal.
